\documentclass{article}
\usepackage[utf8]{inputenc}
\usepackage[english, russian]{babel}
\usepackage[section]{placeins}
%\usepackage{upgreek}
\usepackage{graphicx}
\usepackage{caption}
%\usepackage{subcaption}
\usepackage{wrapfig}
\usepackage{amsmath}
\usepackage{amssymb}
\usepackage{gensymb}
%\usepackage{cyr}
\usepackage{epsf}

\usepackage[top=20mm, bottom=20mm, left=20mm, right=20mm]{geometry}

\title{How many levels is needed in non-stationary regime?}

\begin{document}
\maketitle


\section{Level populations equation}

Level populations can be found by solving the system of equations
\begin{equation}
    \frac{\partial n_i}{\partial t} + \nabla\cdot(n_i \mathbf{v}) = \sigma_i.
\end{equation}
In steady flow in 1D with coordinate \(s\) the equation  becomes
\begin{equation}\label{eq:1d-full}
    \frac{d}{ds}\left(n_i v\right) = v\frac{dn_i}{ds} + n_i\frac{dv}{ds} = \sigma_i
\end{equation}

\section{Sources of hydrogen atom levels populations in 1D case}

Sources of populations for each hydrogen energy level are written as
\begin{equation}\label{eq:sources}
    \begin{aligned}
        \sigma_i &= \sum\limits_{k=i+1}^\infty n_k(A_{ki} + B_{ki}J_{ki}) + \sum\limits_{j=1}^{i-1} n_jB_{ji}J_{ij}+ n_e^2(A_{ci} + WB_{ci})+\\
        &+n_e\left(\sum\limits_{j\neq i}n_jq_{ji}  + n_e^2q_{ci}\right)-\\
        &-n_i\left(\sum\limits_{j=1}^{i-1}(A_{ij} + B_{ij}J_{ij}) + \sum\limits_{k=i+1}^\infty B_{ik}J_{ki} + WB_{ic}\right) -\\
        &-n_in_e\left(q_{ic} + \sum\limits_{i \neq j}q_{ij}\right)
    \end{aligned}
\end{equation}
It's convinient to introduce so called Menzel parameters \(b_i\), defined by
\begin{equation}\label{eq:menzel}
    \frac{n_i}{n_e^2} = b_i\frac{i^2h^3}{(2\pi m_ek_BT_e)^{3/2}}e^{X_i},
\end{equation}
where \(X_j = 13.6\ \mathrm{eV}/(i^2k_BT_e)\). Substituting \(b_i\) in \eqref{eq:sources} and using the relations between collisonal coefficients
\[
\frac{q_{ci}}{q_{ic}} = \frac{i^2h^3}{(2\pi m_ek_BT_e)^{3/2}}e^{X_i}\ \mathrm{and}\  \frac{q_{ul}}{q_{lu}} = \frac{l^2}{u^2}e^{X_l - X_u}
\]
\begin{equation}
    \begin{aligned}
        \frac{(2\pi m_ek_BT_e)^{3/2}}{n_e^2i^2h^3}e^{-X_i}\sigma_i &= \sum\limits_{k=i+1}^\infty b_k\frac{k^2}{i^2}e^{X_k-X_i}(A_{ki} + B_{ki}J_{ki}) + \sum\limits_{j=1}^{i-1} b_j\frac{j^2}{i^2}e^{X_j-X_i}B_{ji}J_{ij} +\\
        &+\frac{(2\pi m_ek_BT_e)^{3/2}}{i^2h^3}e^{-X_i}(A_{ci} + WB_{ci}) +n_e\left(\sum\limits_{j \neq i}(b_j-b_i)q_{ij}  + (1-b_i)q_{ic}\right)-\\
        &-b_i\left(\sum\limits_{j=1}^{i-1}(A_{ij} + B_{ij}J_{ij}) + \sum\limits_{k=i+1}^\infty B_{ik}J_{ki} + WB_{ic}\right) -\\
        &-b_in_e\left(q_{ic} + \sum\limits_{i \neq j}q_{ij}\right)
    \end{aligned}
\end{equation}
Then, applying Sobolev approximation,
\[
J_{ul} = \frac{2h\nu_{ul}^3}{c^2}\left(\overline{S}_{ul}(1-\beta_{lu}) + W\beta_{lu} \overline{I^\star}_{ul}\right),
\]
assuming CFR
\[
\overline{S}_{ul} = \left(\frac{n_l}{n_u}\frac{u^2}{l^2} - 1\right)^{-1} = \left(\frac{b_l}{b_u}e^{X_l-X_u} - 1\right)^{-1}
\]
and black-body star
\[
\overline{I^\star}_{ul} = \left(e^{X_l - X_u} - 1\right)^{-1}
\]
and using relations between einstein coefficients
\[
A_{ul} = \frac{2h\nu_{ul}^3}{c^2}B_{ul}\ \mathrm{and}\ \frac{B_{ul}}{B_{lu}} = \frac{l^2}{u^2},
\]
we get
\begin{equation}\label{eq:sources-bi}
    \begin{aligned}
        \frac{(2\pi m_ek_BT_e)^{3/2}}{n_e^2i^2h^3}e^{-X_i}\sigma_i &= \sum\limits_{k=i+1}^\infty b_k\frac{k^2}{i^2}e^{X_k-X_i}A_{ki}\beta_{ik}(1 + W\overline{I^\star}_{ki}) + \sum\limits_{j=1}^{i-1} b_je^{X_j-X_i}A_{ij}W\beta_{ji} \overline{I^\star}_{ij} +\\
        &+\frac{(2\pi m_ek_BT_e)^{3/2}}{i^2h^3}e^{-X_i}(A_{ci} + WB_{ci}) +n_e\left(\sum\limits_{j \neq i}(b_j-b_i)q_{ij}  + (1-b_i)q_{ic}\right)-\\
        &-b_i\left(\sum\limits_{j=1}^{i-1}A_{ij}\beta_{ji}(1 + W\overline{I^\star}_{ij}) + \sum\limits_{k=i+1}^\infty A_{ki}\frac{k^2}{i^2}W\overline{I^\star}_{ki}\beta_{ik}  + WB_{ic}\right).
    \end{aligned}
\end{equation}

\begin{equation}
    \begin{aligned}
        \sigma_i &= \sum\limits_{k=i+1}^\infty n_kA_{ki}\beta_{ik}(1 + W\overline{I^\star}_{ki}) + \sum\limits_{j=1}^{i-1} n_j\frac{i^2}{j^2}A_{ij}W\beta_{ji} \overline{I^\star}_{ij} +n_e^2(A_{ci} + WB_{ci}) -\\
        &-n_i\left(\sum\limits_{j=1}^{i-1}A_{ij}\beta_{ji}(1 + W\overline{I^\star}_{ij}) + \sum\limits_{k=i+1}^\infty A_{ki}\frac{k^2}{i^2}W\overline{I^\star}_{ki}\beta_{ik}  + WB_{ic}\right) +\\
        &+n_e\left(\sum\limits_{j \neq i}\left(n_j\frac{i^2}{j^2}e^{X_i-X_j}-n_i\right)q_{ij}  + \left(n_e^2\frac{i^2h^3}{(2\pi m_ek_BT_e)^{3/2}}e^{X_i}-n_i\right)q_{ic}\right). 
    \end{aligned}
\end{equation}

To approximately take into account continuum absorbtion we can multiply terms \(n_e^2(A_{ci} + WB_{ci})\) and \(n_iWB_{ci}\) by continuum escape propability \(\beta_{ic}\)
\[
    \beta_{ic} = \frac{1 - e^{-\tau_{ic}}}{\tau_{ic}} = \frac{1 - e^{-k_{ic}n_iz}}{k_{ic}n_iz} 
\] 
where \(k_{ic}\) is computed at the frequency \(\nu_{ci} = 13.6\ \mathrm{eV}/(i^2h)\) and \(z\) is the depth of the medium. So, finally

\begin{equation}
    \begin{aligned}
        \sigma_i &= \sum\limits_{k=i+1}^\infty n_kA_{ki}\beta_{ik}(1 + W\overline{I^\star}_{ki}) + \sum\limits_{j=1}^{i-1} n_j\frac{i^2}{j^2}A_{ij}W\beta_{ji} \overline{I^\star}_{ij} +\beta_{ic}n_e^2(A_{ci} + \beta_{ic}WB_{ci}) -\\
        &-n_i\left(\sum\limits_{j=1}^{i-1}A_{ij}\beta_{ji}(1 + W\overline{I^\star}_{ij}) + \sum\limits_{k=i+1}^\infty A_{ki}\frac{k^2}{i^2}W\overline{I^\star}_{ki}\beta_{ik}  + \beta_{ic}WB_{ic}\right) +\\
        &+n_e\left(\sum\limits_{j \neq i}\left(n_j\frac{i^2}{j^2}e^{X_i-X_j}-n_i\right)q_{ij}  + \left(n_e^2\frac{i^2h^3}{(2\pi m_ek_BT_e)^{3/2}}e^{X_i}-n_i\right)q_{ic}\right). 
    \end{aligned}
\end{equation}


\section{Stationary solution}

From \eqref{eq:sources-bi}, assuming \(\sigma_i = 0\)
\begin{equation}\label{eq:stat-bi}
    \begin{aligned}
        &\sum\limits_{k=i+1}^\infty b_k\frac{k^2}{i^2}e^{X_k-X_i}A_{ki}\beta_{ik}(1 + W\overline{I^\star}_{ki}) + \sum\limits_{j=1}^{i-1} b_je^{X_j-X_i}A_{ij}W\beta_{ji} \overline{I^\star}_{ij} +\\
        &+\frac{(2\pi m_ek_BT_e)^{3/2}}{i^2h^3}e^{-X_i}(A_{ci} + WB_{ci}\beta_{ic})\beta_{ic} +n_e\left(\sum\limits_{j \neq i}(b_j-b_i)q_{ij}  + (1-b_i)q_{ic}\right)-\\
        &-b_i\left(\sum\limits_{j=1}^{i-1}A_{ij}\beta_{ji}(1 + W\overline{I^\star}_{ij}) + \sum\limits_{k=i+1}^\infty A_{ki}\frac{k^2}{i^2}W\overline{I^\star}_{ki}\beta_{ik}  + WB_{ic}\beta_{ic}\right) = 0.
    \end{aligned}
\end{equation}
We can rewrite this as 
\begin{equation}
    \mathcal{M}\mathbf{b} = -\mathbf{R},
\end{equation}
where \(\mathcal{M}\) is a matrix
\begin{equation}
    \begin{aligned}
        \mathcal{M}_{ii} &= -\sum\limits_{j=1}^{i-1}A_{ij}\beta_{ji} - \sum\limits_{i\neq j}^\infty A_{ij}W\overline{I^\star}_{ij}\beta_{ij}  - WB_{ic}\beta_{ic} - n_e\left(\sum\limits_{i\neq j} q_{ij} + q_{ic}\right)\\
        \mathcal{M}_{ul} &= e^{X_u-X_l}A_{lu}\beta_{lu}(1 + W\overline{I^\star}_{ul}) + n_eq_{lu}\\
        \mathcal{M}_{lu} &= e^{X_l-X_u}A_{ul}W\beta_{ul} \overline{I^\star}_{ul} + n_eq_{ul}
    \end{aligned}
\end{equation}
and \(\mathbf{R}\) is a vector
\begin{equation}
    R_i = \frac{(2\pi m_ek_BT_e)^{3/2}}{i^2h^3}e^{-X_i}(A_{ci} + WB_{ci}\beta_{ic})\beta_{ic} + n_eq_{ic}.
\end{equation}
The solution to this system of equations is \(\mathbf{\bar{b}}\), which can be transformed back to level populations \(\mathbf{\bar{n}}\) using
\begin{equation}
    \bar{n}_i = \bar{n}_e^2\bar{b}_i\frac{i^2h^3}{(2\pi m_ek_BT_e)^{3/2}}e^{X_i},
\end{equation}
where \(\bar{n}_e = n_\mathrm{H} - \sum\limits_{i = 1}^{\infty}\bar{n}_i\).

\section{Linear approximation}

Let's asume that temperature \(T_e\) and density \(n_\mathrm{H}\) are slightly perturbed along \(s\)
\begin{equation}
\begin{aligned}
    T_e &= \bar{T}_e + \delta T_e = \bar{T}_e + \tilde{T}_e e^{iks}\\
    n_\mathrm{H} &= \bar{n}_\mathrm{H} + \delta n_\mathrm{H} = \bar{n}_\mathrm{H} + \tilde{n}_\mathrm{H} e^{iks},
\end{aligned}
\end{equation}
and approximate the solution to equation \eqref{eq:1d-full} as
\begin{equation}
n_i = \bar{n}_i + \delta n_i = \bar{n}_i + \tilde{n}_i e^{iks}.
\end{equation}
Thus, equation \eqref{eq:1d-full} can be simlified as
\begin{equation}
    iksv\delta n_i + n_i
\end{equation}

\section{Sources linearization}

\[
\frac{\partial \beta}{\partial \tau} = \frac{e^{-\tau}}{\tau} - \frac{1-e^{-\tau}}{\tau^2} = \frac{1}{\tau} - \frac{1 - e^{-\tau}}{\tau}  - \frac{1 - e^{-\tau}}{\tau^2} = \frac{1-\beta}{\tau} - \beta
\]
Let's define \(\alpha\) as
\[
\frac{\partial \beta}{\partial \tau} = \frac{1-\beta}{\tau} - \beta = \alpha \tau^{-1}
\]

\[
    \tau_{lu} = \frac{c^3A_{ul}}{8\pi |\mathbf{n}\mathbf{\nabla}(\mathbf{v}\mathbf{n})|}\frac{u^2}{l^2} n_l \left(1 - \frac{n_u}{n_l}\frac{l^2}{u^2}\right)
\]

\[
    \delta\tau_{lu} =  \frac{c^3A_{ul}}{8\pi |\mathbf{n}\mathbf{\nabla}(\mathbf{v}\mathbf{n})|}\left( \frac{u^2}{l^2}\delta n_l - \delta n_u \right)
\]

\[
    \delta\beta_{lu} = \frac{\partial \beta_{lu}}{\partial \tau_{lu}} \frac{c^3A_{ul}}{8\pi |\mathbf{n}\mathbf{\nabla}(\mathbf{v}\mathbf{n})|}\left( \frac{u^2}{l^2}\delta n_l - \delta n_u \right) = \alpha_{lu}(n_lu^2 - n_ul^2)^{-1}(u^2\delta n_l - l^2 \delta n_u)
\]


\[
    \delta\sigma_i = \sum\limits_{j = 1}^\infty  \left(\mathfrak{S}_{ij}-\mathfrak{S}[n_\mathrm{H}]\right)\delta n_j + \sum\limits_{P \in \mathcal{P}}\mathfrak{S}_i[P]\delta{P}
\]
\subsection{Radiative terms}
First, let's consider discrete radiative terms:
\begin{equation}
    \begin{aligned}
        \sigma_i &= \sum\limits_{k=i+1}^\infty n_kA_{ki}\beta_{ik}(1 + W\overline{I^\star}_{ki}) + \sum\limits_{j=1}^{i-1} n_j\frac{i^2}{j^2}A_{ij}W\beta_{ji} \overline{I^\star}_{ij} -\\
        &-n_i\left(\sum\limits_{j=1}^{i-1}A_{ij}\beta_{ji}(1 + W\overline{I^\star}_{ij}) + \sum\limits_{k=i+1}^\infty A_{ki}\frac{k^2}{i^2}W\overline{I^\star}_{ki}\beta_{ik}\right)\dots 
    \end{aligned}
\end{equation}
After linearization (multiple steps)
\begin{equation}
    \begin{aligned}
        \mathfrak{S}_{ii} &= \sum\limits_{j=1}^{i-1} A_{ij}(1 + W\overline{I^\star}_{ij})\left(j^2n_i (1 - \beta_{ji} - \beta_{ji}\tau_{ji})(n_ji^2 - n_ij^2)^{-1} -\beta_{ji}\right)\\
        &+\sum\limits_{j=1}^{i-1} n_j\frac{i^2}{j^2}A_{ij}W\overline{I^\star}_{ij}j^2(1 - \beta_{ji} - \beta_{ji}\tau_{ji})(n_ji^2 - n_ij^2)^{-1}\\
        &-\sum\limits_{k=i+1}^\infty A_{ki}\frac{k^2}{i^2}W\overline{I^\star}_{ki}(\beta_{ik} + k^2n_i(1 - \beta_{ik} - \beta_{ik}\tau_{ik})(n_ik^2 - n_ki^2)^{-1})\\
        &+\sum\limits_{k=i+1}^\infty i^2n_kA_{ki}\frac{k^2}{i^2}(1 - \beta_{ik} - \beta_{ik}\tau_{ik})(n_ik^2 - n_ki^2)^{-1}(1 + W\overline{I^\star}_{ki})
    \end{aligned}
\end{equation}
\begin{equation}
    \begin{aligned}
        \mathfrak{S}_{ii} &= \sum\limits_{j=1}^{i-1} A_{ij}W\overline{I^\star}_{ij}j^2n_i (1 - \beta_{ji} - \beta_{ji}\tau_{ji})(n_ji^2 - n_ij^2)^{-1}\\
        &-\sum\limits_{j=1}^{i-1} A_{ij}W\overline{I^\star}_{ij}i^2n_j(1 - \beta_{ji} - \beta_{ji}\tau_{ji})(n_ji^2 - n_ij^2)^{-1}\\
        &+\sum\limits_{j=1}^{i-1} A_{ij}\left(j^2n_i (1 - \beta_{ji} - \beta_{ji}\tau_{ji})(n_ji^2 - n_ij^2)^{-1} -\beta_{ji}-\beta_{ji}W\overline{I^\star}_{ij}\right)\\
        &-\sum\limits_{k=i+1}^\infty A_{ki}\frac{k^2}{i^2}W\overline{I^\star}_{ki}k^2n_i(1 - \beta_{ik} - \beta_{ik}\tau_{ik})(n_ik^2 - n_ki^2)^{-1}\\
        &+\sum\limits_{k=i+1}^\infty i^2n_kA_{ki}\frac{k^2}{i^2}W\overline{I^\star}_{ki}(1 - \beta_{ik} - \beta_{ik}\tau_{ik})(n_ik^2 - n_ki^2)^{-1}\\
        &+\sum\limits_{k=i+1}^\infty i^2n_kA_{ki}\frac{k^2}{i^2}(1 - \beta_{ik} - \beta_{ik}\tau_{ik})(n_ik^2 - n_ki^2)^{-1}-\sum\limits_{k=i+1}^\infty A_{ki}\frac{k^2}{i^2}W\overline{I^\star}_{ki}\beta_{ik}\dots
    \end{aligned}
\end{equation}
\begin{equation}
    \begin{aligned}
        \mathfrak{S}_{ii} &= -\sum\limits_{j=1}^{i-1} A_{ij}W\overline{I^\star}_{ij}(1 - \beta_{ji} - \beta_{ji}\tau_{ji})-\sum\limits_{k=i+1}^\infty A_{ki}\frac{k^2}{i^2}W\overline{I^\star}_{ki}(1 - \beta_{ik} - \beta_{ik}\tau_{ik})\\
        &+\sum\limits_{j=1}^{i-1} A_{ij}\left(j^2n_i (1 - \beta_{ji} - \beta_{ji}\tau_{ji})(n_ji^2 - n_ij^2)^{-1} -\beta_{ji}(1+W\overline{I^\star}_{ij})\right)\\
        &+\sum\limits_{k=i+1}^\infty i^2n_kA_{ki}\frac{k^2}{i^2}(1 - \beta_{ik} - \beta_{ik}\tau_{ik})(n_ik^2 - n_ki^2)^{-1}-\sum\limits_{k=i+1}^\infty A_{ki}\frac{k^2}{i^2}W\overline{I^\star}_{ki}\beta_{ik}\dots
    \end{aligned}
\end{equation}
if we let (assuming \(u > l\))
\[
    A_{lu} = \frac{u^2}{l^2}A_{ul},\ \overline{I^\star}_{lu} = \overline{I^\star}_{ul},\ \overline{S}_{lu} = \overline{S}_{ul} \ \mathrm{and}\ \tau_{ul} = \tau_{lu}
\]
\begin{equation}
    \begin{aligned}
        \mathfrak{S}_{ii} &= \sum\limits_{j \neq i}^{\infty} A_{ij}\left(\alpha_{ji}(\overline{S}_{ij} - W\overline{I^\star}_{ij}) -\beta_{ji}W\overline{I^\star}_{ij}\right) - \sum\limits_{j=1}^{i-1}A_{ij}\beta_{ji}\dots
    \end{aligned}
\end{equation}
\begin{equation}
    \mathfrak{S}_{lu} = A_{ul}(1 + W\overline{I}_{ul})(\alpha_{lu} + \beta_{lu}) - A_{ul}n_lu^2\alpha_{lu}(n_lu^2 - n_ul^2)^{-1}\dots
\end{equation}
\begin{equation}
    \mathfrak{S}_{ul} = A_{ul}\frac{u^2}{l^2}W\overline{I}_{ul}(\alpha_{lu}  + \beta_{lu}) - A_{ul}n_uu^2\alpha_{lu}(n_lu^2 - n_ul^2)^{-1}\dots
\end{equation}
\begin{equation}
    \begin{aligned}
        \mathfrak{S}[W] &= \sum\limits_{j\neq i}^\infty (n_j-n_i)A_{ji}\beta_{ij}\overline{I^\star}_{ji} \ldots
    \end{aligned}\end{equation}
Radiative continuum terms
\[
    \sigma_i = \beta_{ic}(n_e^2(A_{ci} + \beta_{ic}WB_{ci}) - n_iWB_{ic})...
\]
\[
    \delta \beta_{ic} = \alpha_{ic}\left(n_i^{-1}\delta n_i + k_{ic}^{-1}\frac{\partial k_{ic}}{\partial T_e}\delta T_e + z^{-1}\delta z\right)
\]
after linearization
\begin{equation}
    \delta\sigma_i = 2n_e\beta_{ic}(A_{ci} + \beta_{ic}WB_{ci})\delta n_e + (n_e^2(A_{ci} + 2\beta_{ic}WB_{ci}) - n_iWB_{ic})\delta\beta_{ic} - \beta_{ic}WB_{ic}\delta n_i + (n_e^2\beta_{ic}^2B_{ci} - n_iB_{ic})\delta W
\end{equation}
and
\begin{equation}
    \delta n_e = \delta n_\mathrm{H} - \sum\limits_{i=1}^\infty\delta n_i
\end{equation}
So
\begin{equation}
    \begin{aligned}
        \mathfrak{S}_{ii} &= \ldots \alpha_{ic}(n_e^2n_i^{-1}(A_{ci} + 2\beta_{ic}WB_{ci}) - WB_{ic}) - \beta_{ic}WB_{ic}\ldots   \\ 
        \mathfrak{S}[T_e] &= (n_e^2(A_{ci} + 2\beta_{ic}WB_{ci}) - n_iWB_{ic})\alpha_{ic}k_{ic}^{-1}\frac{\partial k_{ic}}{\partial T_e} \ldots\\
        \mathfrak{S}[z] &= (n_e^2(A_{ci} + 2\beta_{ic}WB_{ci}) - n_iWB_{ic})\alpha_{ic}z^{-1} \ldots\\
        \mathfrak{S}[W] &= \ldots (n_e^2\beta_{ic}^2B_{ci} - n_iB_{ic})\\
        \mathfrak{S}[n_\mathrm{H}] &= 2n_e\beta_{ic}(A_{ci} + \beta_{ic}WB_{ci})\ldots
    \end{aligned}
\end{equation}
\subsection{Collisional terms}
From collisional terms
\begin{equation}
    \begin{aligned}
        \delta\sigma_i = \ldots &\left(\sum\limits_{j \neq i}\left(n_j\frac{i^2}{j^2}e^{X_i-X_j}-n_i\right)q_{ij}  + \left(3n_e^2\frac{i^2h^3}{(2\pi m_ek_BT_e)^{3/2}}e^{X_i}-n_i\right)q_{ic}\right)\delta n_e - \\
        & n_e\left(\sum\limits_{i \neq j}q_{ij} + q_{ic}\right)\delta n_i + n_e \sum\limits_{i\neq j}\frac{i^2}{j^2}e^{X_i-X_j}q_{ij}\delta n_j + \\
        & n_e\left(\sum\limits_{j \neq i}\left(n_j\frac{i^2}{j^2}e^{X_i-X_j}-n_i\right)\frac{\partial q_{ij}}{\partial T_e}  + \left(n_e^2\frac{i^2h^3}{(2\pi m_ek_BT_e)^{3/2}}e^{X_i}-n_i\right)\frac{\partial q_{ic}}{\partial T_e}\right)\delta T_e + \\
        & n_eT_e^{-1}\left(\sum\limits_{j \neq i}n_j\frac{i^2}{j^2}e^{X_i-X_j}q_{ij}(X_i - X_j) + n_e^2\frac{i^2h^3}{(2\pi m_ek_BT_e)^{3/2}}e^{X_i}q_{ic}\left(\frac{3}{2} + X_i\right)\right)\delta T_e 
    \end{aligned}
\end{equation}
So
\begin{equation}
    \begin{aligned}
        \mathfrak{S}_{ii} &= \ldots n_e\left(\sum\limits_{i \neq j}q_{ij} + q_{ic}\right)\\
        \mathfrak{S}_{ij} &= \ldots n_e\frac{i^2}{j^2}e^{X_i-X_j}q_{ij}
    \end{aligned}
\end{equation}
and
\begin{equation}
    \begin{aligned}
        \mathfrak{S}[n_\mathrm{H}] = \ldots& \left(\sum\limits_{j \neq i}\left(n_j\frac{i^2}{j^2}e^{X_i-X_j}-n_i\right)q_{ij}  + \left(3n_e^2\frac{i^2h^3}{(2\pi m_ek_BT_e)^{3/2}}e^{X_i}-n_i\right)q_{ic}\right) \\
        \mathfrak{S}[T_e] = \ldots & n_e\left(\sum\limits_{j \neq i}\left(n_j\frac{i^2}{j^2}e^{X_i-X_j}-n_i\right)\frac{\partial q_{ij}}{\partial T_e}  + \left(n_e^2\frac{i^2h^3}{(2\pi m_ek_BT_e)^{3/2}}e^{X_i}-n_i\right)\frac{\partial q_{ic}}{\partial T_e}\right) + \\
        & n_eT_e^{-1}\left(\sum\limits_{j \neq i}n_j\frac{i^2}{j^2}e^{X_i-X_j}q_{ij}(X_i - X_j) + n_e^2\frac{i^2h^3}{(2\pi m_ek_BT_e)^{3/2}}e^{X_i}q_{ic}\left(\frac{3}{2} + X_i\right)\right)
    \end{aligned}
\end{equation}
\newpage

\subsection{Full expression}
Equation:
\begin{equation}
    \begin{aligned}
        \sigma_i &= \sum\limits_{k=i+1}^\infty n_kA_{ki}\beta_{ik}(1 + W\overline{I^\star}_{ki}) + \sum\limits_{j=1}^{i-1} n_j\frac{i^2}{j^2}A_{ij}W\beta_{ji} \overline{I^\star}_{ij} +\beta_{ic}n_e^2(A_{ci} + \beta_{ic}WB_{ci}) -\\
        &-n_i\left(\sum\limits_{j=1}^{i-1}A_{ij}\beta_{ji}(1 + W\overline{I^\star}_{ij}) + \sum\limits_{k=i+1}^\infty A_{ki}\frac{k^2}{i^2}W\overline{I^\star}_{ki}\beta_{ik}  + \beta_{ic}WB_{ic}\right) +\\
        &+n_e\left(\sum\limits_{j \neq i}\left(n_j\frac{i^2}{j^2}e^{X_i-X_j}-n_i\right)q_{ij}  + \left(n_e^2\frac{i^2h^3}{(2\pi m_ek_BT_e)^{3/2}}e^{X_i}-n_i\right)q_{ic}\right). 
    \end{aligned}
\end{equation}
Linearization (\([P],\ P \in \mathcal{P}\) --- variable parameter):
\[
    \delta\sigma_i = \sum\limits_{j = 1}^\infty  \left(\mathfrak{S}_{ij}-\mathfrak{S}[n_\mathrm{H}]\right)\delta n_j + \sum\limits_{P \in \mathcal{P}}\mathfrak{S}_i[P]\delta{P}.
\]
Level populations matrix:
\begin{equation}
    \begin{aligned}
        \mathfrak{S}_{ii} =& \sum\limits_{j \neq i}^{\infty} A_{ij}\left(\alpha_{ji}(\overline{S}_{ij} - W\overline{I^\star}_{ij}) -\beta_{ji}W\overline{I^\star}_{ij}\right) - \sum\limits_{j=1}^{i-1}A_{ij}\beta_{ji} + \\
        &n_e\left(\sum\limits_{i \neq j}q_{ij} + q_{ic}\right) + \alpha_{ic}(n_e^2n_i^{-1}(A_{ci} + 2\beta_{ic}WB_{ci}) - WB_{ic}) - \beta_{ic}WB_{ic}\\
        \mathfrak{S}_{lu} =& A_{ul}(1 + W\overline{I}_{ul})(\alpha_{lu} + \beta_{lu}) - A_{ul}n_lu^2\alpha_{lu}(n_lu^2 - n_ul^2)^{-1} + n_e\frac{l^2}{u^2}e^{X_l-X_u}q_{lu}\\
        \mathfrak{S}_{ul} =& A_{ul}\frac{u^2}{l^2}W\overline{I}_{ul}(\alpha_{lu}  + \beta_{lu}) - A_{ul}n_uu^2\alpha_{lu}(n_lu^2 - n_ul^2)^{-1} + n_e \frac{u^2}{l^2}e^{X_u-X_l}q_{ul}.
    \end{aligned}
\end{equation}
Parameter vectors:
\begin{equation}
    \begin{aligned}
        \mathfrak{S}[z] = &(n_e^2(A_{ci} + 2\beta_{ic}WB_{ci}) - n_iWB_{ic})\alpha_{ic}z^{-1}\\
        \mathfrak{S}[W] = &\sum\limits_{j\neq i}^\infty (n_j-n_i)A_{ji}\beta_{ij}\overline{I^\star}_{ji} + (n_e^2\beta_{ic}^2B_{ci} - n_iB_{ic})\\
        \mathfrak{S}[n_\mathrm{H}] = & \left(\sum\limits_{j \neq i}\left(n_j\frac{i^2}{j^2}e^{X_i-X_j}-n_i\right)q_{ij}  + \left(3n_e^2\frac{i^2h^3}{(2\pi m_ek_BT_e)^{3/2}}e^{X_i}-n_i\right)q_{ic}\right) + \\
        &2n_e\beta_{ic}(A_{ci} + \beta_{ic}WB_{ci})\\
        \mathfrak{S}[T_e] = & n_eT_e^{-1}\left(\sum\limits_{j \neq i}n_j\frac{i^2}{j^2}e^{X_i-X_j}q_{ij}(X_i - X_j) + n_e^2\frac{i^2h^3}{(2\pi m_ek_BT_e)^{3/2}}e^{X_i}q_{ic}\left(\frac{3}{2} + X_i\right)\right)+\\
        & n_e\left(\sum\limits_{j \neq i}\left(n_j\frac{i^2}{j^2}e^{X_i-X_j}-n_i\right)\frac{\partial q_{ij}}{\partial T_e}  + \left(n_e^2\frac{i^2h^3}{(2\pi m_ek_BT_e)^{3/2}}e^{X_i}-n_i\right)\frac{\partial q_{ic}}{\partial T_e}\right) + \\
        & (n_e^2(A_{ci} + 2\beta_{ic}WB_{ci}) - n_iWB_{ic})\alpha_{ic}k_{ic}^{-1}\frac{\partial k_{ic}}{\partial T_e}.
    \end{aligned}
\end{equation}


\end{document}


